LeanFixpoint/VCG/STLC/Semantics.lean
@@ -1,4 +1,4 @@
-import LeanFixpoint.VCG.STLC.Substitution
+import LeanFixpoint.VCG.STLC.Syntax
 
 open STLC
 
